changed consystency and added initial state

Grandpa/src/Protocol/Protocol.v
@@ -39,43 +39,43 @@ Open Scope natWrapper.
 
 (** *Protocol
 
-The main functions of this module are: 
+The main functions of this module are:
   - [get_state_up_to]
   - [voters_round_step]
 
-Of the same importance but no defined in this module is the 
+Of the same importance but no defined in this module is the
   [StateMessages.update_votes] function.
 
-The [get_state_up_to] function is in charge of performing the 
-main loop of the simulation. It just take the 0 state 
-and feed the [voter_round_step] and  [StateMessages.update_votes] functions 
-with the right states for the corresponding [Time] until 
+The [get_state_up_to] function is in charge of performing the
+main loop of the simulation. It just take the 0 state
+and feed the [voter_round_step] and  [StateMessages.update_votes] functions
+with the right states for the corresponding [Time] until
 we reach the desired Time.
 
-At every time [t], we have two stages:  
-  - Update the local state of every voter according to the messages received 
-    by that voter up to this time. 
-  - Proceed to run the Grandpa protocol or to act as a byzantine voter 
+At every time [t], we have two stages:
+  - Update the local state of every voter according to the messages received
+    by that voter up to this time.
+  - Proceed to run the Grandpa protocol or to act as a byzantine voter
     for every voter of the protocol.
 
-The [StateMessages.update_votes] function models the message passing 
-between participants. 
+The [StateMessages.update_votes] function models the message passing
+between participants.
 
-The [voters_round_step] function models the actions of the participants 
+The [voters_round_step] function models the actions of the participants
 at a particular time and global state of the protocol.
 
 See the documentation of each function for details.
 
-Other functions of high interest: 
+Other functions of high interest:
 
-  - [prevoter_step_legit] what a honest prevoter does 
+  - [prevoter_step_legit] what a honest prevoter does
   - [precommit_step_legit] what a honest precommiter does
   - [finalize_block]
 *)
 
 
 (**
-Given a block [b], looks in all the blocks produced by block producer 
+Given a block [b], looks in all the blocks produced by block producer
 for this round and time.
 Filters all the blocks [x] such that [b <=? x].
 And gets the block with the higher block number.
@@ -87,16 +87,16 @@ Definition look_for_best_chain_for_block `{Io} (t:Time) (v:Voter) (ablock:AnyBlo
   in
   let available_blocks := block_producer t v
   in
-  let blocks_that_contains_it := 
-    List.filter 
-    (fun x => AnyBlock.is_prefix ablock  x) 
+  let blocks_that_contains_it :=
+    List.filter
+    (fun x => AnyBlock.is_prefix ablock  x)
     (Sets.to_list available_blocks)
   in
   match blocks_that_contains_it with
   | List.nil => None
   | _ =>
     Some(
-      List.fold_left 
+      List.fold_left
         (fun x y => if (x.(AnyBlock.block_number) <? y.(AnyBlock.block_number))%nat then y else x)
         blocks_that_contains_it
         (AnyBlock.to_any OriginBlock)
@@ -104,21 +104,21 @@ Definition look_for_best_chain_for_block `{Io} (t:Time) (v:Voter) (ablock:AnyBlo
   end.
 
 (**
-Creates a prevote message for the given block, 
+Creates a prevote message for the given block,
 adds it to the local state (to set that the voter already voted),
 and sends the message.
 *)
 Definition build_and_send_prevote
   (t:Time)
-  (state:State) 
-  (voter:Voter) 
+  (state:State)
+  (voter:Voter)
   (vs:VoterState)
   (b:AnyBlock)
   :State
   :=
-      let new_message : Message.Message 
+      let new_message : Message.Message
         :=
-        {| 
+        {|
           id:= Message.from_nat (1 + state.(message_count))
           ;Message.block:=b
           ;kind:=Message.PreVoteMessage
@@ -128,30 +128,30 @@ Definition build_and_send_prevote
           ;processed_by:=Sets.from_list (voter::List.nil)
         |}
       in
-        let 
+        let
           up_prevote := VoterState.update_prevoted vs (Some b)
         in
         let up_round := VoterState.update_votes_with_msg up_prevote new_message
-        in 
+        in
         advance_count
           (update_voter_state (update_message state new_message) voter up_round).
 
 (**
-Creates a precommit message for the given block, 
+Creates a precommit message for the given block,
 adds it to the local state (to set that the voter already voted),
 and sends the message.
 *)
 Definition build_and_send_precommit
   (t:Time)
-  (state:State) 
-  (voter:Voter) 
+  (state:State)
+  (voter:Voter)
   (vs:VoterState)
   (b:AnyBlock)
   :State
   :=
-      let new_message : Message.Message 
+      let new_message : Message.Message
         :=
-        {| 
+        {|
           id:= Message.from_nat (S state.(message_count))
           ;Message.block:=b
           ;kind:=Message.PreCommitMessage
@@ -161,25 +161,25 @@ Definition build_and_send_precommit
           ;processed_by:=Sets.from_list (voter::List.nil)
         |}
       in
-        let 
+        let
           up_precommit := VoterState.update_precommit vs (Some b)
         in
         let up_round := VoterState.update_votes_with_msg up_precommit new_message
-        in 
+        in
         advance_count
           (update_voter_state (update_message state new_message) voter up_round).
 
 Definition build_and_send_primary_estimate
   (t:Time)
-  (state:State) 
-  (voter:Voter) 
+  (state:State)
+  (voter:Voter)
   (vs:VoterState)
   (b:AnyBlock)
   :State
   :=
-      let new_message : Message.Message 
+      let new_message : Message.Message
         :=
-        {| 
+        {|
           id:= Message.from_nat (S state.(message_count))
           ;Message.block:=b
           ;kind:=Message.EstimateMessage
@@ -190,35 +190,35 @@ Definition build_and_send_primary_estimate
         |}
       in
       let updated_voter_state
-        := 
+        :=
         VoterState.update_last_block vs b
       in
         advance_count
-          (update_voter_state 
-            (update_message state new_message) 
+          (update_voter_state
+            (update_message state new_message)
             voter updated_voter_state
           ).
 
 
 (**
-Create a message that the given block is being finalized, 
-adds it to both the local collection of finalized blocks, 
-and the global collection. 
+Create a message that the given block is being finalized,
+adds it to both the local collection of finalized blocks,
+and the global collection.
 Then we send the message.
 *)
 Definition build_and_send_finalized_block
   (t:Time)
-  (state:State) 
-  (voter:Voter) 
+  (state:State)
+  (voter:Voter)
   (vs:VoterState)
   (b:AnyBlock)
   (votes:Message.FinalizeBlock)
   (opaque:OpaqueRound.OpaqueRoundState)
   :State
   :=
-      let new_message : Message.Message 
+      let new_message : Message.Message
         :=
-        {| 
+        {|
           id:= Message.from_nat (S state.(message_count))
           ;Message.block:=b
           ;kind:=Message.FinalizationMessage votes
@@ -229,20 +229,20 @@ Definition build_and_send_finalized_block
         |}
       in
       let updated_voter_state
-        := 
+        :=
         VoterState.update_add_finalized_block vs b
       in
-      let finalized_block := 
+      let finalized_block :=
         FinalizedBlock.make_with_round t voter b opaque
       in
       State.update_add_finalized_block
         (
         advance_count
-          (update_voter_state 
-            (update_message state new_message) 
+          (update_voter_state
+            (update_message state new_message)
             voter updated_voter_state
           )
-        ) 
+        )
         finalized_block.
 
 
@@ -253,19 +253,19 @@ Definition prevoter_step_aux `{Io} (t:Time) (state:State) (voter:Voter) (vs:Vote
   in
   match Vectors.get tower (RoundNumber.to_nat vs.(VoterState.round_number)-1) with
   |Some (OpaqueRound.OpaqueRoundStateC previous_round)
-    => 
-    let ref_block := 
+    =>
+    let ref_block :=
       match vs.(last_brodcasted_block) with
-      | Some b => 
-          match 
+      | Some b =>
+          match
             (g (Round.get_all_prevote_votes previous_round)
               ,Estimate.get_estimate previous_round
             )
           with
           | (Some g_prev, Some estimate_prev)
               =>
-              if 
-                Block.is_prefix estimate_prev.(AnyBlock.block) b.(AnyBlock.block) 
+              if
+                Block.is_prefix estimate_prev.(AnyBlock.block) b.(AnyBlock.block)
                 && Block.is_prefix b.(AnyBlock.block) g_prev.(AnyBlock.block)
               then Some b
               else Estimate.get_estimate previous_round
@@ -273,35 +273,35 @@ Definition prevoter_step_aux `{Io} (t:Time) (state:State) (voter:Voter) (vs:Vote
           end
       | None => Estimate.get_estimate previous_round
       end
-    in 
-    match map (look_for_best_chain_for_block t voter) ref_block with 
+    in
+    match map (look_for_best_chain_for_block t voter) ref_block with
     | Some (Some b) => build_and_send_prevote t state voter vs b
     | _ => state
     end
   | None => state
   end.
 
-Definition prevoter_step_legit `{Io} 
-  (t:Time) 
-  (state:State) 
-  (voter:Voter) 
+Definition prevoter_step_legit `{Io}
+  (t:Time)
+  (state:State)
+  (voter:Voter)
   (category:VoterCategory)
   (vs:VoterState)
   : State
   :=
-  match vs.(prevoted_block) with 
-  | Some _ => state 
+  match vs.(prevoted_block) with
+  | Some _ => state
   | None =>
     let tower := vs.(VoterState.rounds)
     in
     match Vectors.get tower (RoundNumber.to_nat vs.(VoterState.round_number)) with
     | Some (OpaqueRound.OpaqueRoundStateC round_) =>
       match Estimate.try_to_complete_round round_  with
-      | Some _ => 
+      | Some _ =>
           prevoter_step_aux t state voter vs
       | None=>
-          if t<=? Round.get_start_time round_ + (Time.from_nat 2)*global_time_constant 
-          then 
+          if t<=? Round.get_start_time round_ + (Time.from_nat 2)*global_time_constant
+          then
             prevoter_step_aux t state voter vs
           else
             state
@@ -311,53 +311,53 @@ Definition prevoter_step_legit `{Io}
     end
   end.
 
-Definition prevoter_step `{Io} 
-  (t:Time) 
-  (state:State) 
-  (voter:Voter) 
+Definition prevoter_step `{Io}
+  (t:Time)
+  (state:State)
+  (voter:Voter)
   (category:VoterCategory)
   (vs:VoterState)
   : State
   :=
-  match category with 
-  | VoterState.Bizantine 
+  match category with
+  | VoterState.Bizantine
     =>
-    match io_bizantine_vote t voter with 
+    match io_bizantine_vote t voter with
     | Some b => build_and_send_prevote t state voter vs b
     | None => state
     end
-  | VoterState.Honest 
-    => 
+  | VoterState.Honest
+    =>
     prevoter_step_legit t state voter category vs
   end.
 
-Definition precommit_step_legit `{Io} 
-  (t:Time) 
-  (state:State) 
-  (voter:Voter) 
+Definition precommit_step_legit `{Io}
+  (t:Time)
+  (state:State)
+  (voter:Voter)
   (category:VoterCategory)
   (vs:VoterState)
   : State
   :=
   let tower := vs.(VoterState.rounds)
   in
-  match vs.(precommited_block) with 
+  match vs.(precommited_block) with
   | Some _ => state
   | None =>
     match Vectors.get tower (RoundNumber.to_nat vs.(VoterState.round_number)) with
     | Some (OpaqueRound.OpaqueRoundStateC r) =>
       match Vectors.get tower (RoundNumber.to_nat vs.(VoterState.round_number) - 1) with
       | Some (OpaqueRound.OpaqueRoundStateC r_prev) =>
-        match (g (Round.get_all_prevote_votes r), Estimate.get_estimate r_prev) with 
+        match (g (Round.get_all_prevote_votes r), Estimate.get_estimate r_prev) with
         | (Some g_r,Some estimate_prev)
-          => 
+          =>
           (* TODO: add third condition of precommit *)
           if (t <? Round.get_start_time r + (Time.from_nat 4)*global_time_constant)
-            || Estimate.is_completable r 
+            || Estimate.is_completable r
           then
-            build_and_send_precommit t state voter vs g_r 
-          else 
-            state 
+            build_and_send_precommit t state voter vs g_r
+          else
+            state
         | _ => state
         end
       | None => state
@@ -367,64 +367,64 @@ Definition precommit_step_legit `{Io}
     end
   end.
 
-Definition precommit_step `{Io} 
-  (t:Time) 
-  (state:State) 
-  (voter:Voter) 
+Definition precommit_step `{Io}
+  (t:Time)
+  (state:State)
+  (voter:Voter)
   (category:VoterCategory)
   (vs:VoterState)
   : State
   :=
-  match category with 
-  | VoterState.Bizantine 
+  match category with
+  | VoterState.Bizantine
     =>
-    match io_bizantine_vote t voter with 
-    | Some b => 
+    match io_bizantine_vote t voter with
+    | Some b =>
         build_and_send_precommit t state voter vs b
     | None => state
     end
-  | VoterState.Honest 
-    => 
+  | VoterState.Honest
+    =>
     precommit_step_legit t state voter category vs
   end.
 
 Definition get_last_finalized_block_number
-  (finalized_blocks:Sets.DictionarySet AnyBlock)  
+  (finalized_blocks:Sets.DictionarySet AnyBlock)
   : nat
-  := 
-  List.fold_left 
-    (fun acc y => max acc y.(AnyBlock.block_number)) 
+  :=
+  List.fold_left
+    (fun acc y => max acc y.(AnyBlock.block_number))
     (Sets.to_list finalized_blocks)
     0.
 
 (**
-A block $b = g (C_{r,v})$ can be finalized by a voter [v] if : 
+A block $b = g (C_{r,v})$ can be finalized by a voter [v] if :
   - [b] its block number is above the all the finalized blocks the voter knows.
   - [b] has a supermajority in $V_{r,v}$
 *)
 Definition should_finalize
-  (finalized_blocks:Sets.DictionarySet AnyBlock)  
-  (opaque:OpaqueRound.OpaqueRoundState) 
+  (finalized_blocks:Sets.DictionarySet AnyBlock)
+  (opaque:OpaqueRound.OpaqueRoundState)
   : option AnyBlock
   :=
   let max_block_number := get_last_finalized_block_number finalized_blocks
   in
-  match opaque with 
-  | OpaqueRound.OpaqueRoundStateC r 
+  match opaque with
+  | OpaqueRound.OpaqueRoundStateC r
     =>
     match g (Round.get_all_precommit_votes r) with
     | None => None
-    | Some b => 
-      if negb 
+    | Some b =>
+      if negb
         (Sets.or
-          (fun b2 
-            => 
+          (fun b2
+            =>
             (b.(AnyBlock.block_number) <? max_block_number)%nat
-          ) 
+          )
           finalized_blocks
         ) && Votes.block_has_supermajority b (Round.get_all_prevote_votes r)
-      then 
-        Some b 
+      then
+        Some b
       else None
     end
   end.
@@ -441,33 +441,33 @@ Definition get_voter_state (v:Voter) (state:State)
 
 Definition is_voter_for_round `{Io} (v:Voter) (round_number:RoundNumber)
   : bool
-  := 
+  :=
   is_some (get_voter_kind_for_round v round_number).
 
 (**
-All the blocks on all the rounds that a voter can finalize that haven 
+All the blocks on all the rounds that a voter can finalize that haven
 been finalized.
 
 First, we get all the blocks that the current voter knows has been finalized.
-Then get all the rounds in witch the current voter has participated 
+Then get all the rounds in witch the current voter has participated
 until now.
-We inspect every round to see if we can finalize now a block that haven been 
+We inspect every round to see if we can finalize now a block that haven been
 finalized before.
 *)
-Program Definition get_blocks_to_finalize `{Io} (voter:Voter) (vs:VoterState) 
+Program Definition get_blocks_to_finalize `{Io} (voter:Voter) (vs:VoterState)
   : list (OpaqueRound.OpaqueRoundState * AnyBlock)
-  := 
+  :=
   let finalizeds := vs.(VoterState.finalized_blocks)
   in
-  let all_previous_rounds 
+  let all_previous_rounds
     : list OpaqueRound.OpaqueRoundState
-    := 
+    :=
     (
-      VectorDef.to_list 
+      VectorDef.to_list
         (
-          VectorDef.take 
-            (RoundNumber.to_nat vs.(VoterState.round_number)-1) 
-            _ 
+          VectorDef.take
+            (RoundNumber.to_nat vs.(VoterState.round_number)-1)
+            _
             vs.(VoterState.rounds)
         )
     )
@@ -476,16 +476,16 @@ Program Definition get_blocks_to_finalize `{Io} (voter:Voter) (vs:VoterState)
     : OpaqueRound.OpaqueRoundState -> bool
     :=fun opaque => is_voter_for_round voter (OpaqueRound.get_round_number opaque)
   in
-  let filtered_rounds 
+  let filtered_rounds
     : list OpaqueRound.OpaqueRoundState
     := List.filter predicate all_previous_rounds
   in
-  List.fold_left 
-    (fun acc opaque => 
-      match should_finalize finalizeds opaque  with 
-      | Some b => (opaque,b)::acc 
+  List.fold_left
+    (fun acc opaque =>
+      match should_finalize finalizeds opaque  with
+      | Some b => (opaque,b)::acc
       | None => acc end
-    ) 
+    )
     filtered_rounds
     List.nil.
 Next Obligation.
@@ -500,15 +500,15 @@ Made to me used together with get_blocks_to_finalize.
 Take a block and all the info needed to build a [FinalizeBlock],
 then adds it to the finalized_blocks in the global state.
 *)
-Definition finalize_block (t:Time) 
-  (voter:Voter) 
-  (state:State) 
+Definition finalize_block (t:Time)
+  (voter:Voter)
+  (state:State)
   (opaque_and_block:OpaqueRound.OpaqueRoundState * AnyBlock)
   : State
   :=
   match get_voter_state voter state with
-  | Some vs 
-    => 
+  | Some vs
+    =>
     let (opaque,b) := opaque_and_block
     in
     let fin_msg
@@ -523,18 +523,18 @@ Definition finalize_block (t:Time)
     build_and_send_finalized_block t state voter vs b fin_msg opaque
   | None => state
   end.
- 
+
 (**
-Multiple voters may finalize the same block if they notice it can be 
+Multiple voters may finalize the same block if they notice it can be
 finalized but haven't received a finalization message.
 *)
-Definition finalization `{Io} (t:Time) (state:State) 
-  (voter:Voter) (vs:VoterState) 
-  :State 
-  := 
-  List.fold_left 
-    (finalize_block t voter) 
-    (get_blocks_to_finalize voter vs) 
+Definition finalization `{Io} (t:Time) (state:State)
+  (voter:Voter) (vs:VoterState)
+  :State
+  :=
+  List.fold_left
+    (finalize_block t voter)
+    (get_blocks_to_finalize voter vs)
     state.
 
 
@@ -543,8 +543,8 @@ See if the current round is completable and advance to next round in such case.
 If voter is the primary voter, we also broadcast the estimate.
 *)
 Definition wait_step_for_new_round `{Io}
-  (t:Time) 
-  (voter:Voter) 
+  (t:Time)
+  (voter:Voter)
   (vs:VoterState)
   (state:State)
   : State
@@ -555,24 +555,24 @@ Definition wait_step_for_new_round `{Io}
   |Some (OpaqueRound.OpaqueRoundStateC r)
     =>
     match Estimate.try_to_complete_round r with
-    | Some _ => 
-        let new_vs := 
-          State.init_next_round_voter_state_from 
-            (io_get_round_voters 
+    | Some _ =>
+        let new_vs :=
+          State.init_next_round_voter_state_from
+            (io_get_round_voters
               (
                 (RoundNumber.from_nat 1)
-                + 
+                +
                 vs.(VoterState.round_number)
               )
-            ) 
-            t 
+            )
+            t
             vs
         in
-        let updated_state := update_voter_state state voter new_vs 
+        let updated_state := update_voter_state state voter new_vs
         in
         if voter_is_primary_for_round voter vs.(VoterState.round_number)
         then
-          match Estimate.get_estimate r with 
+          match Estimate.get_estimate r with
           | Some b => build_and_send_primary_estimate t state voter vs b
           | None => updated_state
           end
@@ -583,19 +583,19 @@ Definition wait_step_for_new_round `{Io}
   | None => state
   end.
 
-Definition should_wait_for_next_round `{Io} 
-  (t:Time) 
-  (state:State) 
+Definition should_wait_for_next_round `{Io}
+  (t:Time)
+  (state:State)
   (voter:Voter)
   (vs:VoterState)
   : bool
   :=
   match get_voter_kind_for_round voter vs.(VoterState.round_number) with
-  | Some (VoterKindC Bizantine _) => 
+  | Some (VoterKindC Bizantine _) =>
       io_bizantine_advance_round t voter vs.(VoterState.round_number)
-  | Some (VoterKindC _ vote_right) 
+  | Some (VoterKindC _ vote_right)
       =>
-      match vote_right with 
+      match vote_right with
       | VotePrevote
           => is_some vs.(VoterState.prevoted_block)
       | VotePrecommit
@@ -610,12 +610,12 @@ Definition should_wait_for_next_round `{Io}
 
 
 (**
-If the participant (voter) has one of 
+If the participant (voter) has one of
 the following conditions ([should_wait_for_next_round]):
    - Is a byzantine voter wishing to advance round.
    - Is a voter that already fulfilled it's obligations for this round.
    - Isn't a voter for this round.
-We see if the current round (for the voter) is completable and if it is, 
+We see if the current round (for the voter) is completable and if it is,
 we advance the voter local state to a new round. Otherwise do nothing.
 
 Otherwise we get perform the corresponding action for the particular voter
@@ -623,114 +623,114 @@ in the protocol or the byzantine action.
 *)
 Definition voter_round_step_aux `{Io} (t:Time) (state:State) (voter:Voter): State :=
   match get_voter_state voter state with
-  | Some voter_state_ =>  
-      if should_wait_for_next_round t state voter voter_state_ 
+  | Some voter_state_ =>
+      if should_wait_for_next_round t state voter voter_state_
       then wait_step_for_new_round t voter voter_state_ state
       else
-        match 
+        match
           get_voter_kind_for_round voter voter_state_.(VoterState.round_number)
         with
-        | Some(VoterKindC category kind_) => 
+        | Some(VoterKindC category kind_) =>
             match kind_ with
-            | VotePrevote 
-                => 
+            | VotePrevote
+                =>
                 prevoter_step t state voter category voter_state_
-            | VotePrecommit 
-                =>  
+            | VotePrecommit
+                =>
                 precommit_step t state voter category voter_state_
-            | VoteBoth => 
+            | VoteBoth =>
                 match voter_state_.(VoterState.prevoted_block) with
-                | Some _ => 
+                | Some _ =>
                   match voter_state_.(VoterState.precommited_block) with
                   (* this shouldn't happen! thanks to the first check *)
                   |Some _ => state
                   |None =>
                     precommit_step t state voter category voter_state_
                   end
-                | None => 
+                | None =>
                   prevoter_step t state voter category voter_state_
                 end
             end
-        | _ => state 
+        | _ => state
         end
   (*This shouldn't happen, we set all participants at the begining!*)
   | _ => state
   end.
 
 (**
-First we attempt to finalize all the blocks that we see as finalized but 
+First we attempt to finalize all the blocks that we see as finalized but
 that aren't still finalized by some one.
 
-Then we really perform the Grandpa protocol or the byzantiner actions for 
+Then we really perform the Grandpa protocol or the byzantiner actions for
 this time.
 *)
 (*TODO:
-If this function is called by the members of voters_round_step, 
-the lookup for the voter must be always a Some. This is guaranteed by 
-the facts in the Io class and the way we construct the states. 
-We may add a theorem stating this. 
+If this function is called by the members of voters_round_step,
+the lookup for the voter must be always a Some. This is guaranteed by
+the facts in the Io class and the way we construct the states.
+We may add a theorem stating this.
 *)
 Definition voter_round_step `{Io} (t:Time) (state:State) (voter:Voter): State :=
   match get_voter_state voter state with
-  | Some vs =>  
-    voter_round_step_aux 
-      t 
+  | Some vs =>
+    voter_round_step_aux
+      t
       (finalization t state voter vs)
       voter
   | None => state
   end.
 
-(** 
+(**
 This function models the grandpa protocol together with byzantine voters.
 
-If a particular participant is byzantine in a round, they send messages 
-as dictated by the functions in Io. 
+If a particular participant is byzantine in a round, they send messages
+as dictated by the functions in Io.
 
 If a participant is honest in a round, it follows the grandpa protocol.
 
-This function expect to be run after a votes update. 
-This means that all participants of the model have received all the 
+This function expect to be run after a votes update.
+This means that all participants of the model have received all the
 messages that they are supposed to receive at this time.
 
-As we separate the process of reception of votes/messages from the emission 
-of them, we can update every voter local state independently. 
+As we separate the process of reception of votes/messages from the emission
+of them, we can update every voter local state independently.
 This update for a single voter is done in [voter_round_step].
 *)
 Definition voters_round_step `{Io} (t:Time) (state:State): State :=
   let voters := List.map fst (Dictionary.to_list state.(voters_state))
-  in 
+  in
     List.fold_left (voter_round_step t) voters state .
 
 
-Fixpoint get_state_up_to_nat_aux `{Io} (n:nat) (state_0:State) 
-  : State 
+Fixpoint get_state_up_to_nat_aux `{Io} (n:nat) (state_0:State)
+  : State
   :=
-  match n with 
+  match n with
   | 0 => state_0
-  | S m 
-    => 
+  | S m
+    =>
     let old_state := get_state_up_to_nat_aux m state_0
     in
-    voters_round_step 
-      (Time.from_nat n) 
+    voters_round_step
+      (Time.from_nat n)
       (update_votes (Time.from_nat n) old_state)
   end.
 
-Definition get_state_up_to `{Io} (t:Time) : State 
-  :=
-  let 
+Definition initial_state `{io:Io} :State :=
+  let
     zero_round_dict := io_get_round_voters (RoundNumber.from_nat 0)
   in
-  let 
-    state_0 :=  State.make_initial_state_from zero_round_dict
-  in
-  get_state_up_to_nat_aux (Time.to_nat t) state_0.
+  State.make_initial_state_from zero_round_dict.
+
+Definition get_state_up_to `{Io} (t:Time) : State
+  :=
+  get_state_up_to_nat_aux (Time.to_nat t) initial_state.
 
 
 (*
 This takes some time to compute, but it eventually does.
-We believe the reason is that no Io instance is provide and the 
-computation must be made abstract. As such, we end with a 300k 
+We believe the reason is that no Io instance is provide and the
+computation must be made abstract. As such, we end with a 300k
 lines result instead of a simple State.
 *)
 (* Compute get_state_up_to (Time.from_nat 1).*)
