Grandpa/src/Protocol/Proofs/Consistency/Finalization.v
@@ -1,0 +1,69 @@
+Require Import Blocks.AnyBlock.
+Require Import Voters.
+Require Import Preliminars.
+Require Estimate.
+Require OpaqueRound.
+Require Round.
+Require Import Time.
+Require Import RoundNumber.
+Require Import VoterState.
+Require Import Vectors.
+Require Import Sets.
+Require Import Message.
+Require Import DataTypes.List.Count.
+Require Import DataTypes.List.Fold.
+Require Import DataTypes.Option.
+Require Import Protocol.State.
+Require Import Protocol.StateMessages.
+Require Import Protocol.FinalizedBlock.
+Require Import Protocol.Protocol.
+
+Require Import Classes.Functor.
+Require Import Classes.Eqb.
+Require Import Classes.Math.All.
+Require Import Instances.List.
+
+
+Require Import Protocol.Io.
+Require Import Protocol.
+
+Section ProtocolFinalizationConsistency.
+
+Open Scope bool.
+Open Scope list.
+Open Scope eqb.
+Open Scope math.
+Open Scope natWrapper.
+
+
+
+Theorem all_voters_verify_finalization `{io:Io}
+  (fb:FinalizedBlock)
+  (v:Voter)
+  (v_participates_in_protocol:
+    exists vs,  get_voter_state v initial_state = Some vs)
+  :
+  let t_min := (fb.(FinalizedBlock.time) +  ((Time.from_nat 2) * global_time_constant) )
+  in
+  let r_n := fb.(FinalizedBlock.round_number)
+  in
+  forall t,
+  t >= t_min ->
+  let state := get_state_up_to t
+  in
+  (exists r, get_voter_opaque_round state v r_n = Some r
+    /\
+      Votes.block_has_supermajority
+        fb.(FinalizedBlock.block)
+        (OpaqueRound.get_all_prevote_votes r)
+      = true
+  ).
+  (*TODO: critical
+  Proof by stating the same thing but only for t_min
+  and use the fact that the rounds are monotone (ie
+     they grow over time and are consistent with
+     previous states
+   *)
+  Admitted.
+
+End ProtocolFinalizationConsistency.
